thys/Untyped_Lambda_Calculus/ILC.thy
@@ -496,99 +496,95 @@ by (meson Un_bound card_of_subset_bound imsupp_supp_bound infinite_ivar s(2) sin
 lemma SSupp_rrename_update_bound:
 assumes s[simp]: "bij (\<sigma>::ivar\<Rightarrow>ivar)" "|supp \<sigma>| <o |UNIV::ivar set|"
 shows "|SSupp (rrename \<sigma> \<circ> iVar(x := e))| <o |UNIV::ivar set|"
-using IImsupp_rrename_update_bound[OF assms] unfolding IImsupp_def  apply auto
-HERE
-(* 
-  by (smetis (mono_tags) IImsupp_def finite_Un finite_iff_le_card_var)
+using IImsupp_rrename_update_bound[OF assms] unfolding IImsupp_def  
+using SSupp_rrename_bound s(1) s(2) by auto 
 
 (* Action of swapping (a particular renaming) on variables *)
 
-lemma rrename_swap_Var1[simp]: "rrename (id(x := xx, xx := x)) (Var (x::var)) = Var xx"
+lemma rrename_swap_Var1[simp]: "rrename (id(x := xx, xx := x)) (iVar (x::ivar)) = iVar xx"
 apply(subst rrename_simps(1)) by auto
-lemma rrename_swap_Var2[simp]: "rrename (id(x := xx, xx := x)) (Var (xx::var)) = Var x"
+lemma rrename_swap_Var2[simp]: "rrename (id(x := xx, xx := x)) (iVar (xx::ivar)) = iVar x"
 apply(subst rrename_simps(1)) by auto
-lemma rrename_swap_Var3[simp]: "z \<notin> {x,xx} \<Longrightarrow> rrename (id(x := xx, xx := x)) (Var (z::var)) = Var z"
+lemma rrename_swap_Var3[simp]: "z \<notin> {x,xx} \<Longrightarrow> rrename (id(x := xx, xx := x)) (iVar (z::ivar)) = iVar z"
 apply(subst rrename_simps(1)) by auto
-lemma rrename_swap_Var[simp]: "rrename (id(x := xx, xx := x)) (Var (z::var)) =
- Var (if z = x then xx else if z = xx then x else z)"
+lemma rrename_swap_Var[simp]: "rrename (id(x := xx, xx := x)) (iVar (z::ivar)) =
+ iVar (if z = x then xx else if z = xx then x else z)"
 apply(subst rrename_simps(1)) by auto
 
 (* Compositionality properties of renaming and term-for-variable substitution *)
 
 lemma itvsubst_comp:
-assumes s[simp]: "|SSupp \<sigma>| <o |UNIV:: var set|" "|SSupp \<tau>| <o |UNIV:: var set|"
-shows "itvsubst (\<sigma>::var\<Rightarrow>trm) (itvsubst \<tau> e) = itvsubst (itvsubst \<sigma> \<circ> \<tau>) e"
+assumes s[simp]: "|SSupp \<sigma>| <o |UNIV:: ivar set|" "|SSupp \<tau>| <o |UNIV:: ivar set|"
+shows "itvsubst (\<sigma>::ivar\<Rightarrow>itrm) (itvsubst \<tau> e) = itvsubst (itvsubst \<sigma> \<circ> \<tau>) e"
 proof-
   note SSupp_itvsubst_bound'[OF s, simp]
   show ?thesis
-  apply(induct e rule: term.fresh_induct[where A = "IImsupp \<sigma> \<union> IImsupp \<tau>"])
+  apply(induct e rule: iterm.fresh_induct[where A = "IImsupp \<sigma> \<union> IImsupp \<tau>"])
     subgoal using Un_bound[OF s]
       using var_ID_class.Un_bound SSupp_IImsupp_bound s(1) s(2) by blast
     subgoal by simp
-    subgoal by simp
-    subgoal for x t apply(subgoal_tac "x \<notin> IImsupp (\<lambda>a. itvsubst \<sigma> (\<tau> a))")
-      subgoal by simp
+    subgoal by simp (metis (mono_tags, lifting) comp_apply stream.map_comp stream.map_cong)
+    subgoal for xs t apply(subgoal_tac "sset xs \<inter> IImsupp (\<lambda>a. itvsubst \<sigma> (\<tau> a)) = {}")
+      subgoal by simp (metis Int_Un_emptyI1 Int_Un_emptyI2 assms(1) assms(2) iterm.subst(3))
       subgoal using IImsupp_itvsubst_su'[OF s(1)] by blast . .
 qed
 
 lemma rrename_itvsubst_comp:
-assumes b[simp]: "bij (\<sigma>::var\<Rightarrow>var)" and s[simp]: "|supp \<sigma>| <o |UNIV:: var set|" "|SSupp \<tau>| <o |UNIV:: var set|"
+assumes b[simp]: "bij (\<sigma>::ivar\<Rightarrow>ivar)" and s[simp]: "|supp \<sigma>| <o |UNIV:: ivar set|" "|SSupp \<tau>| <o |UNIV:: ivar set|"
 shows "rrename \<sigma> (itvsubst \<tau> e) = itvsubst (rrename \<sigma> \<circ> \<tau>) e"
 proof-
   note SSupp_rrename_bound'[OF b s, simp]
   show ?thesis
-  apply(induct e rule: term.fresh_induct[where A = "IImsupp \<tau> \<union> imsupp \<sigma>"])
-    subgoal using s(1) s(2) Un_bound SSupp_IImsupp_bound imsupp_supp_bound infinite_var by blast
+  apply(induct e rule: iterm.fresh_induct[where A = "IImsupp \<tau> \<union> imsupp \<sigma>"])
+    subgoal using s(1) s(2) Un_bound SSupp_IImsupp_bound imsupp_supp_bound infinite_ivar by blast
     subgoal by simp
-    subgoal by simp
-    subgoal for x t apply simp apply(subgoal_tac "x \<notin> IImsupp (\<lambda>a. rrename  \<sigma> (\<tau> a))")
-      subgoal unfolding imsupp_def supp_def by simp
+    subgoal by simp (metis (mono_tags, lifting) comp_apply stream.map_comp stream.map_cong)
+    subgoal for xs t apply simp apply(subgoal_tac "sset xs \<inter> IImsupp (\<lambda>a. rrename  \<sigma> (\<tau> a)) = {}")
+      subgoal by simp (metis Int_Un_emptyI1 Int_Un_emptyI2 assms(2) b iterm.map(3) iterm.subst(3) iterm_vvsubst_rrename s(2)) 
       subgoal using IImsupp_rrename_su' b s(1) by blast . .
 qed
 
 (* Equivariance of unary substitution: *)
 
 lemma itvsubst_rrename_comp[simp]:
-assumes s[simp]: "bij (\<sigma>::var\<Rightarrow>var)" "|supp \<sigma>| <o |UNIV::var set|"
-shows "itvsubst (rrename \<sigma> \<circ> Var(x := e2)) e1 = itvsubst (Var(\<sigma> x := rrename \<sigma> e2)) (rrename \<sigma> e1)"
+assumes s[simp]: "bij (\<sigma>::ivar\<Rightarrow>ivar)" "|supp \<sigma>| <o |UNIV::ivar set|"
+shows "itvsubst (rrename \<sigma> \<circ> iVar(x := e2)) e1 = itvsubst (iVar(\<sigma> x := rrename \<sigma> e2)) (rrename \<sigma> e1)"
 proof-
   note SSupp_rrename_update_bound[OF assms, unfolded comp_def, simplified, simp]
   note SSupp_update_rrename_bound[unfolded fun_upd_def, simplified, simp]
   show ?thesis
-  apply(induct e1 rule: term.fresh_induct[where A = "{x} \<union> FFVars_term e2 \<union> imsupp \<sigma>"])
-    subgoal by (meson Un_bound imsupp_supp_bound infinite_var s(2) singl_bound term.set_bd_UNIV)
+  apply(induct e1 rule: iterm.fresh_induct[where A = "{x} \<union> FFVars e2 \<union> imsupp \<sigma>"])
+    subgoal by (meson Un_bound imsupp_supp_bound infinite_ivar s(2) singl_bound iterm.set_bd_UNIV)
     subgoal by auto
-    subgoal by simp
-    subgoal for y t apply simp apply(subgoal_tac
-      "y \<notin> IImsupp ((\<lambda>a. rrename \<sigma> (if a = x then e2 else Var a))) \<and>
-      \<sigma> y \<notin> IImsupp (\<lambda>a. if a = \<sigma> x then rrename \<sigma> e2 else Var a)")
-      subgoal unfolding imsupp_def supp_def by simp
-      subgoal unfolding IImsupp_def imsupp_def SSupp_def supp_def by auto . .
+    subgoal by simp (smt (verit, best) comp_apply stream.map_comp stream.map_cong)
+    subgoal for ys t apply simp apply(subgoal_tac
+      "sset ys \<inter> IImsupp ((\<lambda>a. rrename \<sigma> (if a = x then e2 else iVar a))) = {} \<and>
+      \<sigma> ` sset ys \<inter>  IImsupp (\<lambda>a. if a = \<sigma> x then rrename \<sigma> e2 else iVar a) = {}")
+      subgoal by simp (metis (no_types, lifting) Int_Un_emptyI2 imsupp_empty_IntD2 stream.map_ident_strong)  
+      subgoal unfolding IImsupp_def imsupp_def SSupp_def supp_def by (auto split: if_splits)  . .
 qed
 
 (* Unary substitution versus swapping: *)
 lemma itvsubst_Var_rrename:
-assumes xx: "xx \<notin> FFVars_term e1 - {x}"
-shows "itvsubst (Var((x::var) := e2)) e1 = itvsubst (Var(xx := e2)) (rrename (id(x := xx, xx := x)) e1)"
+assumes xx: "xx \<notin> FFVars e1 - {x}"
+shows "itvsubst (iVar((x::ivar) := e2)) e1 = itvsubst (iVar(xx := e2)) (rrename (id(x := xx, xx := x)) e1)"
 proof-
   show ?thesis using xx
-  apply(induct e1 rule: term.fresh_induct[where A = "{x,xx} \<union> FFVars_term e2"])
-    subgoal by (metis insert_is_Un term.set(1) term.set(2) term.set_bd_UNIV)
+  apply(induct e1 rule: iterm.fresh_induct[where A = "{x,xx} \<union> FFVars e2"])
+    subgoal by (metis insert_is_Un iterm.set_bd_UNIV singl_bound var_iterm_pre_class.Un_bound)
     subgoal by simp
-    subgoal by auto
-    subgoal for y t apply simp apply(subgoal_tac
-      "y \<notin> IImsupp (Var(x := e2)) \<and> y \<notin> IImsupp (Var(xx := e2))")
-      subgoal unfolding imsupp_def supp_def by auto
+    subgoal by simp (smt (verit, best) comp_apply stream.map_comp stream.map_cong) 
+    subgoal for ys t apply simp apply(subgoal_tac
+      "sset ys \<inter> IImsupp (iVar(x := e2)) = {} \<and> sset ys \<inter> IImsupp (iVar(xx := e2)) = {}")
+      subgoal by simp (metis (mono_tags, lifting) SSupp_upd_iVar_bound fun_upd_other iterm.subst(3) stream.map_cong stream.map_id)  
       subgoal unfolding IImsupp_def imsupp_def SSupp_def supp_def by auto . .
 qed
-
-(*   *)
 
 (* *)
 
 (* Swapping and unary substitution, as abbreviations: *)
-abbreviation "swap t (x::var) y \<equiv> rrename (id(x:=y,y:=x)) t"
-abbreviation "usub t (y::var) x \<equiv> vvsubst (id(x:=y)) t"
+abbreviation "swap t (x::ivar) y \<equiv> rrename (id(x:=y,y:=x)) t"
+abbreviation "usub t (y::ivar) x \<equiv> ivvsubst (id(x:=y)) t"
 
 (* *)
 
@@ -596,40 +592,41 @@ lemma usub_swap_disj:
 assumes "{u,v} \<inter> {x,y} = {}"
 shows "usub (swap t u v) x y = swap (usub t x y) u v"
 proof-
-  note term_vvsubst_rrename[simp del]
+  note iterm_vvsubst_rrename[simp del]
   show ?thesis using assms
-  apply(subst term_vvsubst_rrename[symmetric]) apply auto
-  apply(subst term.map_comp) apply auto
-  apply(subst term_vvsubst_rrename[symmetric]) apply auto
-  apply(subst term.map_comp) apply auto
-  apply(rule term.map_cong0)
-    using term_pre.supp_comp_bound by auto
+  apply(subst iterm_vvsubst_rrename[symmetric]) apply auto
+  apply(subst iterm.map_comp) apply auto
+  apply(subst iterm_vvsubst_rrename[symmetric]) apply auto
+  apply(subst iterm.map_comp) apply auto
+  apply(rule iterm.map_cong0)
+  using iterm_pre.supp_comp_bound by auto
 qed
 
 lemma rrename_o_swap:
-"rrename (id(y::var := yy, yy := y) o id(x := xx, xx := x)) t =
+"rrename (id(y::ivar := yy, yy := y) o id(x := xx, xx := x)) t =
  swap (swap t x xx) y yy"
-apply(subst term.rrename_comps[symmetric])
+apply(subst iterm.rrename_comps[symmetric])
 by auto
 
 (* *)
 
-lemma swap_simps[simp]: "swap (Var z) (y::var) x = Var (sw z y x)"
-"swap (App t s) (y::var) x = App(swap t y x) (swap s y x)"
-"swap (Abs v t) (y::var) x = Abs (sw v y x) (swap t y x)"
-by (auto simp: sw_def)
+lemma swap_simps[simp]: "swap (iVar z) (y::ivar) x = iVar (sw z y x)"
+"swap (iApp t ss) (y::ivar) x = iApp (swap t y x) (smap (\<lambda>s. swap s y x) ss)"
+"swap (iAbs vs t) (y::ivar) x = iAbs (smap (\<lambda>v. sw v y x) vs) (swap t y x)"
+unfolding sw_def by simp_all (metis eq_id_iff fun_upd_apply)
 
-lemma FFVars_swap[simp]: "FFVars (swap t y x) =
- (\<lambda>u. sw u x y) ` (FFVars t)"
-apply(subst term.FFVars_rrenames) by (auto simp: sw_def)
+lemma FFVars_swap[simp]: "FFVars (swap t y x) = (\<lambda>u. sw u x y) ` (FFVars t)"
+apply(subst iterm.FFVars_rrenames) by (auto simp: sw_def)
 
-lemma FFVars_swap'[simp]: "{x::var,y} \<inter> FFVars t = {} \<Longrightarrow> swap t x y = t"
-apply(rule term.rrename_cong_ids) by auto
+lemma FFVars_swap'[simp]: "{x::ivar,y} \<inter> FFVars t = {} \<Longrightarrow> swap t x y = t"
+apply(rule iterm.rrename_cong_ids) by auto
 
 (* *)
 
-lemma Abs_inject_swap: "Abs v t = Abs v' t' \<longleftrightarrow>
-  (v' \<notin> FFVars t \<or> v' = v) \<and> swap t v' v = t'"
+thm rrename_cong
+
+lemma iAbs_inject_swap: "iAbs vs t = iAbs vs' t' \<longleftrightarrow>
+  (vs' \<inter> FFVars t = {} \<or> vs' = vs) \<and> map swap t v' v = t'"
 unfolding Abs_inject apply(rule iffI)
   subgoal unfolding id_on_def apply auto
   apply(rule rrename_cong) by auto
